Back-translation of variables and solve all assumptions in back-translation

state/TargetLangHS.fst
@@ -7,27 +7,39 @@ open FStar.Tactics.Typeclasses
 open FStar.HyperStack
 open FStar.HyperStack.ST 
 
-type rref (t:Type) = r:(reference t){not (is_mm r)} (* type of unfreeable heap references allocated in regions *)
+type rref (t:Type) = r:(reference t){
+    not (is_mm r) /\
+    is_eternal_region (frameOf r)} (* type of unfreeable heap references allocated in regions *)
 
 (** target_lang is a shallow embedding of STLC **)
 class target_lang (t:Type) = {
   dcontains : t -> mem -> Type0;
-  regional : t -> mem -> rid -> Type0;
+  has_frame : t -> rid -> Type0; (** shallow check of the region of a value **)
+  regional : t -> mem -> rid -> Type0; (** deep check of the region of a value **)
+  deep_recall : (r:t) -> Stack unit 
+              (requires (fun h -> True))
+              (ensures  (fun h0 _ h1 -> h0 == h1 /\ r `dcontains` h1))
 }
 
 instance target_lang_unit : target_lang unit = {
   dcontains = (fun _ _ -> True);
+  has_frame = (fun _ _ -> True);
   regional = (fun _ _ _ -> True);
+  deep_recall = (fun _ -> ())
 }
 
 instance target_lang_int : target_lang int = {
   dcontains = (fun _ _ -> True);
+  has_frame = (fun _ _ -> True);
   regional = (fun _ _ _ -> True);
+  deep_recall = (fun _ -> ());
 }
 
 instance target_lang_pair (t1:Type) (t2:Type) {| c1:target_lang t1 |} {| c2:target_lang t2 |} : target_lang (t1 * t2) = {
   dcontains = (fun (x1, x2) h -> c1.dcontains x1 h /\ c2.dcontains x2 h);
+  has_frame = (fun (x1, x2) rr -> c1.has_frame x1 rr /\ c2.has_frame x2 rr);
   regional = (fun (x1, x2) h rr -> c1.regional x1 h rr /\ c2.regional x2 h rr);
+  deep_recall = (fun (x1, x2) -> c1.deep_recall x1; c2.deep_recall x2)
 }
 
 instance target_lang_sum (t1:Type) (t2:Type) {| c1:target_lang t1 |} {| c2:target_lang t2 |} : target_lang (either t1 t2) = {
@@ -35,15 +47,29 @@ instance target_lang_sum (t1:Type) (t2:Type) {| c1:target_lang t1 |} {| c2:targe
     match x with
     | Inl x1 -> c1.dcontains x1 h
     | Inr x2 -> c2.dcontains x2 h);
+  has_frame = (fun x rr ->
+    match x with
+    | Inl x1 -> c1.has_frame x1 rr
+    | Inr x2 -> c2.has_frame x2 rr);
   regional = (fun x h rr ->
     match x with
     | Inl x1 -> c1.regional x1 h rr
     | Inr x2 -> c2.regional x2 h rr);
+  deep_recall = (fun x ->
+    match x with
+    | Inl x1 -> c1.deep_recall x1
+    | Inr x2 -> c2.deep_recall x2)
 }
 
 instance target_lang_ref (t:Type) {| c:target_lang t |} : target_lang (rref t) = {
   dcontains = (fun (x:rref t) h -> h `contains` x /\ c.dcontains (sel h x) h);
+  has_frame = (fun (x:rref t) rr -> frameOf x == rr);
   regional = (fun (x:rref t) h rr -> frameOf x == rr /\ c.regional (sel h x) h rr);  
+  deep_recall = (fun (x:rref t) ->
+    recall x;
+    let v = !x in
+    c.deep_recall v 
+  )
 }
 
 let self_contained_region_inv (rr:rid) (h:mem) : Type0 =
@@ -54,10 +80,10 @@ unfold let pre_tgt_arrow
   (rrs:rid)
   (#t1:Type) (x:t1) {| tgtx:target_lang t1 |}
   (h0:mem) =
-  regional x h0 rrs /\                                                     (* x is in region rs *)
+  regional x h0 rrs /\                                                    (* x is deeply in region rs *)
   dcontains x h0 /\                                                       (* required to instantiate the properties of modifies *)
   self_contained_region_inv rrs h0 /\
-  is_eternal_region rrs                                                    (* required for using ralloc *)
+  is_eternal_region rrs                                                   (* required for using ralloc *)
 
 let post_tgt_arrow
   (rrs:rid)
@@ -69,7 +95,7 @@ let post_tgt_arrow
   // equal_dom h0 h1 /\                                                  (* no dynamic allocation *)
   self_contained_region_inv rrs h1 /\
 
-  ((tgtr x).regional r h1 rrs) /\
+  ((tgtr x).regional r h1 rrs) /\                                        (* x is deeply in region rs *)
   ((tgtr x).dcontains r h1)
 (* TODO: what prevents the computation to allocate things in rp? *)
 
@@ -92,7 +118,9 @@ instance target_lang_arrow
   {| (x:t1 -> target_lang (t2 x)) |}
   : target_lang (mk_tgt_arrow rrs t1 t2) = {
     dcontains = (fun _ _ -> True);
+    has_frame = (fun _ _ -> True);
     regional = (fun _ _ _ -> True);
+    deep_recall = (fun _ -> ())
   }
 
 open STLC
@@ -356,12 +384,61 @@ let progr4 #_ #rs #rrs #rrp f =
   ()
 
 (** *** Elaboration of expressions to F* *)
-type vcontext (rs:rid) (g:context) = x:var{Some? (g x)} -> elab_typ (Some?.v (g x)) rs
+let rec regional_implies_has_frame #rrs #t (x:elab_typ t rrs)
+: Stack unit
+    (requires (fun h0 ->
+      (elab_typ_tgt t rrs).regional x h0 rrs))
+    (ensures (fun h0 _ h1 -> h0 == h1 /\
+      (elab_typ_tgt t rrs).has_frame x rrs))
+= match t with
+  | TArr t1 t2 -> ()
+  | TUnit -> ()
+  | TNat -> ()
+  | TSum t1 t2 -> begin
+      let x : either (elab_typ t1 rrs) (elab_typ t2 rrs) = x in
+      match x with 
+      | Inl x1 -> regional_implies_has_frame x1
+      | Inr x2 -> regional_implies_has_frame x2
+  end
+  | TPair t1 t2 -> begin
+      let (x1, x2) : (elab_typ t1 rrs * elab_typ t2 rrs) = x in
+      regional_implies_has_frame x1;
+      regional_implies_has_frame x2
+  end
+  | TRef t -> begin
+      let x : rref (elab_typ t rrs) = x in
+      ()
+  end
 
-let vempty (rs:rid) : vcontext rs empty = fun _ -> assert false
 
-let vextend #t #rs (x:elab_typ t rs) (#g:context) (ve:vcontext rs g) : vcontext rs (extend t g) =
-  fun y -> if y = 0 then x else ve (y-1)
+
+let rec deep_recall_implies_regional #rrs #t (x:elab_typ t rrs)
+: Stack unit
+    (requires (fun h0 ->
+      (elab_typ_tgt t rrs).has_frame x rrs /\
+      (elab_typ_tgt t rrs).dcontains x h0 /\
+      self_contained_region_inv rrs h0))
+    (ensures (fun h0 _ h1 -> h0 == h1 /\
+      (elab_typ_tgt t rrs).regional x h1 rrs))
+= match t with
+  | TArr t1 t2 -> ()
+  | TUnit -> ()
+  | TNat -> ()
+  | TSum t1 t2 -> begin
+      let x : either (elab_typ t1 rrs) (elab_typ t2 rrs) = x in
+      match x with 
+      | Inl x1 -> deep_recall_implies_regional x1
+      | Inr x2 -> deep_recall_implies_regional x2
+  end
+  | TPair t1 t2 -> begin
+      let (x1, x2) : (elab_typ t1 rrs * elab_typ t2 rrs)= x in
+      deep_recall_implies_regional x1;
+      deep_recall_implies_regional x2
+  end
+  | TRef t -> begin
+      let x : rref (elab_typ t rrs) = x in
+      ()
+  end
 
 val elab_apply_arrow :
   rrs:rid ->
@@ -376,7 +453,15 @@ let elab_apply_arrow rs t1 t2 f x = f x
 unfold let elab_typ' rrs t = elab_typ t rrs
 unfold let elab_typ_tgt' rrs t = elab_typ_tgt t rrs
 
-#set-options "--split_queries always"
+type vcontext (rs:rid) (g:context) = 
+  vx:var{Some? (g vx)} -> x:(elab_typ (Some?.v (g vx)) rs){(elab_typ_tgt (Some?.v (g vx)) rs).has_frame x rs}
+
+let vempty (rs:rid) : vcontext rs empty = fun _ -> assert false
+
+let vextend #t #rs (x:(elab_typ t rs){(elab_typ_tgt t rs).has_frame x rs}) (#g:context) (ve:vcontext rs g) : vcontext rs (extend t g) =
+  fun y -> if y = 0 then x else ve (y-1)
+
+#push-options "--split_queries always --z3rlimit 100"
 let rec elab_exp 
   (rrs:rid)
   (#g:context)
@@ -402,20 +487,27 @@ let rec elab_exp
     let r : ref (elab_typ t) = elab_exp tyj_e ve in
     !r
   end
+
   | TyWriteRef #_ #_ #_ #t tyj_ref tyj_v -> begin
       let r : ref (elab_typ t) = elab_exp tyj_ref ve in // <-- this is effectful and modifies fp
       let v : elab_typ t = elab_exp tyj_v ve in // this is effectul and modifies fp
       recall r;
       write' #_ #(elab_typ_tgt t) r v
   end
-  
+
+  | TyVar vx -> 
+    let Some tx = g vx in
+    let x : elab_typ tx = ve vx in
+    (elab_typ_tgt tx).deep_recall x;
+    deep_recall_implies_regional #rrs #tx x;
+    x
   | TyApp #_ #_ #_ #tx #tres tyj_f tyj_x ->
     assert ((elab_typ t) == (elab_typ tres));
     let x : elab_typ tx = elab_exp tyj_x ve in
+    regional_implies_has_frame #rrs #tx x;
     let f : elab_typ (TArr tx tres) = elab_exp tyj_f ve in
-    let h1 = get () in
-    assume ((elab_typ_tgt tx).dcontains x h1); (* TODO: we need to recall x here *)
-    assume ((elab_typ_tgt tx).regional x h1 rrs);
+    (elab_typ_tgt tx).deep_recall x;
+    deep_recall_implies_regional #rrs #tx x;
     elab_apply_arrow rrs tx tres f x
 
   | TyInl #_ #_ #t1 #t2 tyj_1 ->
@@ -428,17 +520,17 @@ let rec elab_exp
     let vc : either (elab_typ tl) (elab_typ tr) = elab_exp tyj_c ve in
     match vc with 
     | Inl x -> 
-        let f : elab_typ (TArr tl tres) = elab_exp tyj_l ve in
-        let h1 = get () in
-        assume ((elab_typ_tgt tl).dcontains x h1); (* TODO: we need to recall x here *)
-        assume ((elab_typ_tgt tl).regional x h1 rrs);
-        elab_apply_arrow rrs tl tres f x
+      regional_implies_has_frame #rrs #tl x;
+      let f : elab_typ (TArr tl tres) = elab_exp tyj_l ve in
+      (elab_typ_tgt tl).deep_recall x;
+      deep_recall_implies_regional #rrs #tl x;
+      elab_apply_arrow rrs tl tres f x
     | Inr y ->
-        let f : elab_typ (TArr tr tres) = elab_exp tyj_r ve in
-        let h1 = get () in
-        assume ((elab_typ_tgt tr).dcontains y h1); (* TODO: recall y *)
-        assume ((elab_typ_tgt tr).regional y h1 rrs);
-        elab_apply_arrow rrs tr tres f y
+      regional_implies_has_frame #rrs #tr y;
+      let f : elab_typ (TArr tr tres) = elab_exp tyj_r ve in
+      (elab_typ_tgt tr).deep_recall y;
+      deep_recall_implies_regional #rrs #tr y;
+      elab_apply_arrow rrs tr tres f y
   end
 
   | TyFst #_ #_ #tf #ts tyj_e ->
@@ -449,10 +541,11 @@ let rec elab_exp
     snd #(elab_typ tf) #(elab_typ ts) v
   | TyPair #_ #_ #_ #tf #ts tyj_f tyj_s->
     let vf : elab_typ tf = elab_exp tyj_f ve in
+    regional_implies_has_frame #rrs #tf vf;
     let vs : elab_typ ts = elab_exp tyj_s ve in
-    let h1 = get () in
-    assume ((elab_typ_tgt tf).dcontains vf h1); (* TODO: recall vf *)
-    assume ((elab_typ_tgt tf).regional vf h1 rrs);
+    (elab_typ_tgt tf).deep_recall vf;
+    deep_recall_implies_regional #rrs #tf vf;
     (vf, vs)
 
   | _ -> admit ()
+  #pop-options
